Lib.Sequence changes

lib/Lib.Sequence.fsti
@@ -16,133 +16,6 @@ let seq (a:Type0) = s:Seq.seq a
 (** Length of a Sequence *)
 let length (#a:Type0) (s:seq a) : nat = Seq.length s
 
-(** Access to an element of a Sequence *)
-val index: #a:Type -> s:seq a -> n:nat{length s > 0 /\ n < length s} -> a
-
-(** Concatenation of two Sequences *)
-val concat:#a:Type -> s1:seq a -> s2:seq a -> r:seq a{length r == length s1 + length s2}
-
-(** Operator for concatenation of two Sequences*)
-let (@|) #a s1 s2 = concat #a s1 s2
-
-(** Equality of two Sequences *)
-abstract
-type equal (#a:Type) (s1:seq a) (s2:seq a) =
- length s1 == length s2 /\
- (forall (i:nat{i < length s1}).{:pattern (index s1 i); (index s2 i)} index s1 i == index s2 i)
-
-(** Lemma on equality of two Sequences *)
-val eq_intro:
-    #a:Type
-  -> s1:seq a
-  -> s2:seq a
-  -> Lemma
-    (requires (length s1 == length s2 /\ (forall (i:nat{i < length s1}).{:pattern (index s1 i); (index s2 i)} index s1 i == index s2 i)))
-    (ensures  (equal s1 s2))
-  [SMTPat (equal s1 s2)]
-
-(** Lemma on equality of two Sequences *)
-val eq_elim:
-    #a:Type
-  -> s1:seq a
-  -> s2:seq a
-  -> Lemma
-    (requires equal s1 s2)
-    (ensures  s1 == s2)
-  [SMTPat (equal s1 s2)]
-
-(* The following functions on unbounded sequences should not be needed in normal crypto specs.
-   Maybe we should leave them in the .fst and not expose them here. *)
-
-(** Updating an element of un unbounded Sequence *)
-val seq_upd:
-    #a:Type
-  -> s:seq a
-  -> n:nat{n < length s}
-  -> x:a
-  -> o:seq a{length o == length s /\ index o n == x /\ (forall (i:nat).
-    {:pattern (index s i)} (i < length s /\ i <> n) ==> index o i == index s i)}
-
-(** Selecting a subset of an unbounded Sequence *)
-val seq_sub:
-    #a:Type
-  -> s1:seq a
-  -> start:nat
-  -> n:nat{start + n <= length s1}
-  -> s2:seq a{length s2 == n /\
-	     (forall (k:nat{k < n}). {:pattern (index s2 k)} index s2 k == index s1 (start + k))}
-
-(** Updating a subset of an unbounded Sequence with another Sequence *)
-val seq_update_sub:
-    #a:Type
-  -> i:seq a
-  -> start:nat
-  -> n:nat{start + n <= length i}
-  -> x:seq a{length x == n}
-  -> o:seq a{length o == length i /\ seq_sub o start n == x /\
-    (forall (k:nat{(0 <= k /\ k < start) \/ (start + n <= k /\ k < length i)}).
-      {:pattern (index o k)} index o k == index i k)}
-
-(** Lemma on update of a sub-Sequence *)
-val lemma_seq_update_sub:
-    #a:Type
-  -> dst:seq a
-  -> start:nat
-  -> n:nat{start + n <= length dst}
-  -> src:seq a
-  -> res:seq a
-  -> Lemma
-    (requires
-      length res == length dst /\
-      length src == n /\
-      seq_sub res 0 start == seq_sub dst 0 start /\
-      seq_sub res start n == src /\
-      seq_sub res (start + n) (length dst - start - n) ==
-      seq_sub dst (start + n) (length dst - start - n))
-    (ensures
-      res == seq_update_sub dst start n src)
-
-(** Creation of a Sequence from an initial value *)
-val seq_create:
-    #a:Type
-  -> len:nat
-  -> init:a
-  -> s:seq a{length s == len /\ (forall (i:nat).
-    {:pattern (index s i)} i < len ==> index s i == init)}
-
-(** Creation of a Sequence from a list of values *)
-val seq_of_list:
-    #a:Type
-  -> l:list a
-  -> s:seq a{length s == List.Tot.length l}
-
-val seq_of_list_index:
-    #a:Type
-  -> l:list a
-  -> i:nat{i < List.Tot.length l}
-  -> Lemma (index (seq_of_list l) i == List.Tot.index l i)
-    [SMTPat (index (seq_of_list l) i)]
-
-(** Map function for Sequences *)
-val seq_map:#a:Type -> #b:Type -> (a -> Tot b) -> s1:seq a -> s2:seq b{length s2 == length s1}
-
-(** Map2 function for Sequences *)
-val seq_map2:#a:Type -> #b:Type -> #c:Type
-  -> f:(a -> b -> Tot c)
-  -> s1:seq a
-  -> s2:seq b{length s1 == length s2}
-  -> s3:seq c{length s3 == length s2}
-
-(** Forall function for Sequences *)
-val seq_for_all:#a:Type -> (a -> Tot bool) -> seq a -> bool
-
-(** Forall2 function for Sequences *)
-val seq_for_all2:#a:Type -> #b:Type
-  -> (a -> b -> Tot bool)
-  -> s1:seq a
-  -> s2:seq b{length s1 == length s2}
-  -> bool
-
 /// Bounded Sequences
 
 (* This is the type of bounded sequences.
@@ -150,7 +23,14 @@ val seq_for_all2:#a:Type -> #b:Type
    It adds additional length checks that you'd have to prove in the implementation otherwise *)
 
 (** Definition of a fixed-length Sequence *)
-let lseq (a:Type0) (len:size_nat) = s:seq a{(* len > 0 /\*) Seq.length s == len}
+let lseq (a:Type0) (len:size_nat) = s:seq a{Seq.length s == len}
+
+val index:
+    #a:Type
+  -> #len:size_nat
+  -> s:lseq a len
+  -> i:size_nat{i < len}
+  -> a
 
 (** Creation of a fixed-length Sequence from an initial value *)
 val create:
@@ -160,14 +40,25 @@ val create:
   -> s:lseq a len{(forall (i:nat).
     {:pattern (index s i)} i < len ==> index s i == init)}
 
+(** Concatenate sequences: use with care, may make implementation hard to verify *)
+val concat:
+    #a:Type
+  -> #len0:size_nat
+  -> #len1:size_nat{len0 + len1 <= max_size_t}
+  -> s0:lseq a len0
+  -> s1:lseq a len1
+  -> s2:lseq a (len0 + len1)
+
+
 (** Conversion from Sequence to fixed-length Sequence *)
 let to_lseq (#a:Type0) (s:seq a{length s <= max_size_t}) : l:lseq a (length s){l == s} = s
 
 (** Conversion of a Sequence to a list *)
 val to_list:
     #a:Type
-  -> s:seq a
-  -> l:list a{List.Tot.length l = length s}
+  -> #len:size_nat
+  -> s:lseq a len
+  -> l:list a{List.Tot.length l = len}
 
 (** Creation of a fixed-length Sequence from a list of values *)
 val of_list:
@@ -197,7 +88,7 @@ val upd:
 
 (** Operator for accessing an element of a fixed-length Sequence *)
 unfold
-let op_String_Access #a = index #a
+let op_String_Access #a #len = index #a #len
 
 (** Operator for updating an element of a fixed-length Sequence *)
 unfold
@@ -246,10 +137,10 @@ val lemma_update_sub:
   -> res:lseq a len
   -> Lemma
     (requires
-      seq_sub res 0 start == seq_sub dst 0 start /\
+      sub res 0 start == sub dst 0 start /\
       sub res start n == src /\
-      seq_sub res (start + n) (length dst - start - n) ==
-      seq_sub dst (start + n) (length dst - start - n))
+      sub res (start + n) (length dst - start - n) ==
+      sub dst (start + n) (length dst - start - n))
     (ensures
       res == update_sub dst start n src)
 
