lib/fst/Lib.Sequence.fst
@@ -6,31 +6,91 @@ open Lib.LoopCombinators
 
 #set-options "--z3rlimit 15"
 
+(** Access to an element of a Sequence *)
+val seq_index: #a:Type -> s:seq a -> n:nat{length s > 0 /\ n < length s} -> a
+let seq_index #a s n = Seq.index s n
 
-let index #a s n = Seq.index s n
-let concat #a s1 s2 =
+(** Concatenation of two Sequences *)
+val seq_concat:#a:Type -> s1:seq a -> s2:seq a -> r:seq a{length r == length s1 + length s2}
+
+let seq_concat #a s1 s2 =
   let r = (Seq.append s1 s2 <: seq a) in
   assert (length r == length s1 + length s2);
   r
+(** Operator for concatenation of two Sequences*)
+let (@|) #a s1 s2 = seq_concat #a s1 s2
 
+(** Equality of two Sequences *)
+abstract
+type equal (#a:Type) (s1:seq a) (s2:seq a) =
+ length s1 == length s2 /\
+ (forall (i:nat{i < length s1}).{:pattern (seq_index s1 i); (seq_index s2 i)} seq_index s1 i == seq_index s2 i)
+
+(** Lemma on equality of two Sequences *)
+val eq_intro:
+    #a:Type
+  -> s1:seq a
+  -> s2:seq a
+  -> Lemma
+    (requires (length s1 == length s2 /\ (forall (i:nat{i < length s1}).{:pattern (seq_index s1 i); (seq_index s2 i)} seq_index s1 i == seq_index s2 i)))
+    (ensures  (equal s1 s2))
+  [SMTPat (equal s1 s2)]
 let eq_intro #a s1 s2 =
   assert (forall (i:nat{i < length s1}).{:pattern (Seq.index s1 i); (Seq.index s2 i)}
-    index s1 i == index s2 i);
+    seq_index s1 i == seq_index s2 i);
   Seq.lemma_eq_intro #a s1 s2
 
+(** Lemma on equality of two Sequences *)
+val eq_elim:
+    #a:Type
+  -> s1:seq a
+  -> s2:seq a
+  -> Lemma
+    (requires equal s1 s2)
+    (ensures  s1 == s2)
+  [SMTPat (equal s1 s2)]
 let eq_elim #a s1 s2 =
   assert (length s1 == length s2);
   assert (forall (i:nat{i < length s1}).{:pattern (Seq.index s1 i); (Seq.index s2 i)}
-    index s1 i == index s2 i);
+    seq_index s1 i == seq_index s2 i);
   Seq.lemma_eq_elim #a s1 s2
 
+(* The following functions on unbounded sequences should not be needed in normal crypto specs.
+   Maybe we should leave them in the .fst and not expose them here. *)
+
+(** Updating an element of un unbounded Sequence *)
+val seq_upd:
+    #a:Type
+  -> s:seq a
+  -> n:nat{n < length s}
+  -> x:a
+  -> o:seq a{length o == length s /\ seq_index o n == x /\ (forall (i:nat).
+    {:pattern (seq_index s i)} (i < length s /\ i <> n) ==> seq_index o i == seq_index s i)}
 let seq_upd #a s n x = Seq.upd #a s n x
 
+(** Selecting a subset of an unbounded Sequence *)
+val seq_sub:
+    #a:Type
+  -> s1:seq a
+  -> start:nat
+  -> n:nat{start + n <= length s1}
+  -> s2:seq a{length s2 == n /\
+	     (forall (k:nat{k < n}). {:pattern (seq_index s2 k)} seq_index s2 k == seq_index s1 (start + k))}
 let seq_sub #a s start n =
   let r = Seq.slice #a s start (start + n) in
   assert (length r == n);
   r
 
+(** Updating a subset of an unbounded Sequence with another Sequence *)
+val seq_update_sub:
+    #a:Type
+  -> i:seq a
+  -> start:nat
+  -> n:nat{start + n <= length i}
+  -> x:seq a{length x == n}
+  -> o:seq a{length o == length i /\ seq_sub o start n == x /\
+    (forall (k:nat{(0 <= k /\ k < start) \/ (start + n <= k /\ k < length i)}).
+      {:pattern (seq_index o k)} seq_index o k == seq_index i k)}
 let seq_update_sub #a s start n x =
   let o =
     Seq.append
@@ -39,6 +99,24 @@ let seq_update_sub #a s start n x =
   Seq.lemma_eq_intro (Seq.slice o start (start + n)) x;
   o
 
+(** Lemma on update of a sub-Sequence *)
+val lemma_seq_update_sub:
+    #a:Type
+  -> dst:seq a
+  -> start:nat
+  -> n:nat{start + n <= length dst}
+  -> src:seq a
+  -> res:seq a
+  -> Lemma
+    (requires
+      length res == length dst /\
+      length src == n /\
+      seq_sub res 0 start == seq_sub dst 0 start /\
+      seq_sub res start n == src /\
+      seq_sub res (start + n) (length dst - start - n) ==
+      seq_sub dst (start + n) (length dst - start - n))
+    (ensures
+      res == seq_update_sub dst start n src)
 let lemma_seq_update_sub #a dst start n src res =
   let res1 = seq_update_sub dst start n src in
   FStar.Seq.Properties.lemma_split (seq_sub res 0 (start + n)) start;
@@ -46,13 +124,34 @@ let lemma_seq_update_sub #a dst start n src res =
   FStar.Seq.Properties.lemma_split res (start + n);
   FStar.Seq.Properties.lemma_split res1 (start + n)
 
+(** Creation of a Sequence from an initial value *)
+val seq_create:
+    #a:Type
+  -> len:nat
+  -> init:a
+  -> s:seq a{length s == len /\ (forall (i:nat).
+    {:pattern (seq_index s i)} i < len ==> seq_index s i == init)}
 let seq_create #a len init = Seq.create #a len init
 
+(** Creation of a Sequence from a list of values *)
+val seq_of_list:
+    #a:Type
+  -> l:list a
+  -> s:seq a{length s == List.Tot.length l}
 let seq_of_list #a l = Seq.seq_of_list #a l
 
+val seq_of_list_index:
+    #a:Type
+  -> l:list a
+  -> i:nat{i < List.Tot.length l}
+  -> Lemma (seq_index (seq_of_list l) i == List.Tot.index l i)
+    [SMTPat (seq_index (seq_of_list l) i)]
 let seq_of_list_index #a l i =
   Seq.lemma_seq_of_list_index #a l i
 
+
+(** Map function for Sequences *)
+val seq_map:#a:Type -> #b:Type -> (a -> Tot b) -> s1:seq a -> s2:seq b{length s2 == length s1}
 let seq_map #a #b f s =
   Seq.seq_of_list (List.Tot.map f (Seq.seq_to_list s))
 
@@ -65,19 +164,38 @@ let rec map2_list #a #b #c f l1 l2 =
   | [], [] -> []
   | x::l1', y::l2' -> f x y :: map2_list f l1' l2'
 
+
+(** Map2 function for Sequences *)
+val seq_map2:#a:Type -> #b:Type -> #c:Type
+  -> f:(a -> b -> Tot c)
+  -> s1:seq a
+  -> s2:seq b{length s1 == length s2}
+  -> s3:seq c{length s3 == length s2}
 let seq_map2 #a #b #c f s1 s2 =
   Seq.seq_of_list (map2_list f (Seq.seq_to_list s1) (Seq.seq_to_list s2))
 
+(** Forall function for Sequences *)
+val seq_for_all:#a:Type -> (a -> Tot bool) -> seq a -> bool
 let seq_for_all #a f x = Seq.for_all f x
 
+(** Forall2 function for Sequences *)
+val seq_for_all2:#a:Type -> #b:Type
+  -> (a -> b -> Tot bool)
+  -> s1:seq a
+  -> s2:seq b{length s1 == length s2}
+  -> bool
 let seq_for_all2 #a #b f x y =
   let r = seq_map2 (fun xi yi -> f xi yi) x y in
   seq_for_all (fun bi -> bi = true) r
 
 
-let create #a len init = seq_create #a len init
+let index #a #len s n = seq_index s n
 
-let to_list #a s = Seq.Properties.seq_to_list s
+let create #a len init = Seq.create #a len init
+
+let concat #a #len0 #len1 s0 s1 = seq_concat s0 s1
+
+let to_list #a #len s = Seq.Properties.seq_to_list s
 
 let of_list #a l = seq_of_list #a l
 
